<?xml version="1.0"?>
<rdf:RDF xmlns="http://purl.obolibrary.org/obo/opl/dev/import_RO.owl#"
     xml:base="http://purl.obolibrary.org/obo/opl/dev/import_RO.owl"
     xmlns:obo="http://purl.obolibrary.org/obo/"
     xmlns:owl="http://www.w3.org/2002/07/owl#"
     xmlns:rdf="http://www.w3.org/1999/02/22-rdf-syntax-ns#"
     xmlns:xml="http://www.w3.org/XML/1998/namespace"
     xmlns:xsd="http://www.w3.org/2001/XMLSchema#"
     xmlns:rdfs="http://www.w3.org/2000/01/rdf-schema#">
    <owl:Ontology rdf:about="http://purl.obolibrary.org/obo/opl/dev/import_RO.owl"/>
    


    <!-- 
    ///////////////////////////////////////////////////////////////////////////////////////
    //
    // Annotation properties
    //
    ///////////////////////////////////////////////////////////////////////////////////////
     -->

    


    <!-- http://purl.obolibrary.org/obo/IAO_0000115 -->

    <owl:AnnotationProperty rdf:about="http://purl.obolibrary.org/obo/IAO_0000115"/>
    


    <!-- http://purl.obolibrary.org/obo/IAO_0000412 -->

    <owl:AnnotationProperty rdf:about="http://purl.obolibrary.org/obo/IAO_0000412"/>
    


    <!-- http://purl.obolibrary.org/obo/RO_0001900 -->

    <owl:AnnotationProperty rdf:about="http://purl.obolibrary.org/obo/RO_0001900">
        <obo:IAO_0000115>An assertion that holds between an OWL Object Property and a temporal interpretation that elucidates how OWL Class Axioms that use this property are to be interpreted in a temporal context.</obo:IAO_0000115>
        <rdfs:label xml:lang="en">temporal interpretation</rdfs:label>
    </owl:AnnotationProperty>
    


    <!-- http://purl.obolibrary.org/obo/RO_0002416 -->

    <owl:AnnotationProperty rdf:about="http://purl.obolibrary.org/obo/RO_0002416">
        <obo:IAO_0000115>An assertion that involves at least one OWL object that is intended to be expanded into one or more logical axioms. The logical expansion can yield axioms expressed using any formal logical system, including, but not limited to OWL2-DL.</obo:IAO_0000115>
        <rdfs:label xml:lang="en">logical macro assertion</rdfs:label>
    </owl:AnnotationProperty>
    


    <!-- http://purl.obolibrary.org/obo/RO_0002421 -->

    <owl:AnnotationProperty rdf:about="http://purl.obolibrary.org/obo/RO_0002421">
        <obo:IAO_0000115>A logical macro assertion whose domain is an IRI for a property</obo:IAO_0000115>
        <rdfs:label xml:lang="en">logical macro assertion on a property</rdfs:label>
    </owl:AnnotationProperty>
    


    <!-- http://purl.obolibrary.org/obo/RO_0002422 -->

    <owl:AnnotationProperty rdf:about="http://purl.obolibrary.org/obo/RO_0002422">
        <obo:IAO_0000115>Used to annotate object properties to describe a logical meta-property or characteristic of the object property.</obo:IAO_0000115>
        <rdfs:label xml:lang="en">logical macro assertion on an object property</rdfs:label>
    </owl:AnnotationProperty>
    


    <!-- 
    ///////////////////////////////////////////////////////////////////////////////////////
    //
    // Object Properties
    //
    ///////////////////////////////////////////////////////////////////////////////////////
     -->

    


    <!-- http://purl.obolibrary.org/obo/RO_0002160 -->

    <owl:ObjectProperty rdf:about="http://purl.obolibrary.org/obo/RO_0002160">
        <rdfs:subPropertyOf rdf:resource="http://purl.obolibrary.org/obo/RO_0002320"/>
        <obo:IAO_0000115>x only in taxon y if and only if x is in taxon y, and there is no other organism z such that y!=z a and x is in taxon z.</obo:IAO_0000115>
        <obo:IAO_0000412 rdf:resource="http://purl.obolibrary.org/obo/ro.owl"/>
        <rdfs:label rdf:datatype="http://www.w3.org/2001/XMLSchema#string">only in taxon</rdfs:label>
    </owl:ObjectProperty>
    


    <!-- http://purl.obolibrary.org/obo/RO_0002320 -->

    <owl:ObjectProperty rdf:about="http://purl.obolibrary.org/obo/RO_0002320">
        <obo:IAO_0000115>A relationship that holds via some environmental process</obo:IAO_0000115>
        <obo:IAO_0000412 rdf:resource="http://purl.obolibrary.org/obo/ro.owl"/>
        <rdfs:label xml:lang="en">evolutionarily related to</rdfs:label>
    </owl:ObjectProperty>
    


    <!-- http://purl.obolibrary.org/obo/RO_0002321 -->

    <owl:ObjectProperty rdf:about="http://purl.obolibrary.org/obo/RO_0002321">
        <obo:IAO_0000115>A relationship that is mediated in some way by the environment or environmental feature (ENVO:00002297)</obo:IAO_0000115>
        <obo:IAO_0000412 rdf:resource="http://purl.obolibrary.org/obo/ro.owl"/>
        <rdfs:label xml:lang="en">ecologically related to</rdfs:label>
    </owl:ObjectProperty>
    


    <!-- http://purl.obolibrary.org/obo/RO_0002454 -->

    <owl:ObjectProperty rdf:about="http://purl.obolibrary.org/obo/RO_0002454">
        <rdfs:subPropertyOf rdf:resource="http://purl.obolibrary.org/obo/RO_0002321"/>
        <obo:IAO_0000115>X &apos;has host&apos; y if and only if: x is an organism, y is an organism, and x can live on the surface of or within the body of y</obo:IAO_0000115>
        <obo:IAO_0000412 rdf:resource="http://purl.obolibrary.org/obo/ro.owl"/>
        <rdfs:label>has host</rdfs:label>
    </owl:ObjectProperty>
    


    <!-- http://purl.obolibrary.org/obo/RO_0002460 -->

    <owl:ObjectProperty rdf:about="http://purl.obolibrary.org/obo/RO_0002460">
        <rdfs:subPropertyOf rdf:resource="http://purl.obolibrary.org/obo/RO_0002321"/>
        <obo:IAO_0000412 rdf:resource="http://purl.obolibrary.org/obo/ro.owl"/>
        <rdfs:label>has vector</rdfs:label>
    </owl:ObjectProperty>
</rdf:RDF>



<!-- Generated by the OWL API (version 4.5.6) https://github.com/owlcs/owlapi -->

